#CONCEPTS 

## Language generated by a grammar

The language generated by a grammar is a set of strings that can be <span style="color:#db7093;">derivated</span> or <span style="color:#db7093;">generated</span> from a certain grammar. 

The language generated by a grammar <span style="color:MediumSlateBlue;">G</span> is a subset formally defined by: 

$$L(G)= \{W | W ∈ ∑^*, S ⇒ G W\}$$

### Language construction

If considering the following grammar: 

$$G = (N = \{S, A, B\} T = \{a, b\} P = \{S ⇒ AB, A ⇒ aA|a, B ⇒ bB|b\} )$$

The accepted strips can be:
* `ab`
* `abb`
* `aab`
* `aabb`
So the language is:    $L(G) = \{a^m b^n | m ≥ 1\ and\ n ≥ 1\}$

This language can be written from decomposing the different production rules and analyze its individuals patters and the patters combined with other ones. 

### Grammars equivalency

Two grammars $G_0$ and $G_1$ are equivalent if both represents the same language. 

<span style="color:orange;">ontology</span>: given a linear grammar by the right, exist a linear grammar by the left equivalent and viceversa (Type 3).

Example: 

$G_a$ =( {0, 1} ,{A, B}, A,{A ::= B1 | 1,B ::= A0}) 
$G_b$ =( {0, 1} ,{A, B}, A,{A ::= 1B | 1,B ::= 0A})


### Transform direction of linearity

The linearity can be from the right or from the left. 

To transform from one to another, can be done following this steps: 

* Build a grammar non-recursive with the axiom

For doing this, add a new symbol. 
If add a new rule, B ::= x for each rule S ::= x equivalent. So if S ::= A1 --> B ::= A1. 
And replace S axiom in the right part of the production rules with the new rule. 

![[grammar-non-recursive-transformation.png|350]]

* Build a graph from the grammar

`Number of nodes` like  $num\_nodes = C(∑_N)+1$ with each node labeled with $∑_N$ symbols and another with λ for a terminal only replacement. 

![[grammar-graph-construction.png|350]]

![[grammar-graph-construction-2.png|400]]
* Exchange labels and build a new graph

Exchange S and λ labels and invert lines direction. Generate new rules following the graph. 

![[graph-exchange.png|400]]

Then by using the resulting graph, it can be used to build the different <span style="color:#ababf5;">production rules</span> of the new grammar. 

The $∑_T$ and $∑_N$ are still the same as the original grammar, and now the axiom is the new $S$. 


